theories/Factor_Generation_Predecessor_Admission.thy
@@ -1,0 +1,249 @@
+theory Factor_Generation_Predecessor_Admission
+  imports Factor_Generation_Source_Admission
+begin
+
+section \<open>Child operation contracts retain their complete independent domains\<close>
+
+abbreviation generation_child_value_result :: "factor_term \<Rightarrow> bool" where
+  "generation_child_value_result t \<equiv> \<exists>E e u s d H h.
+    t=context_relation_argument (Pair_Term e (use_data_term u)) (address_pair_data (s,d)) h \<and>
+    environment_value_presents E e \<and> octets_formed s \<and> generation_value_presents H h \<and>
+    generation_child_at E u (s,d) H"
+
+theorem generation_child_value_exact:
+  "(149,t)\<in>positive_meaning generation_source_system \<longleftrightarrow> generation_child_value_result t"
+  using generation_core_report_at_source
+  by (auto simp: generation_child_value_equation; blast)
+
+abbreviation generation_child_row_result :: "factor_term \<Rightarrow> bool" where
+  "generation_child_row_result t \<equiv> \<exists>E e u s d v a H row.
+    t=context_relation_argument (Pair_Term e (use_data_term u)) (address_pair_data (s,d)) row \<and>
+    environment_value_presents E e \<and> generation_predecessor_row_presents (s,(d,((v,a),H))) row \<and>
+    located_at E u d v a \<and> generation_at E v a H"
+
+theorem generation_child_row_exact:
+  "(153,t)\<in>positive_meaning generation_source_system \<longleftrightarrow> generation_child_row_result t"
+proof
+  assume holds: "(153,t)\<in>positive_meaning generation_source_system"
+  obtain E e u s d v a h where fields:
+    "t=context_relation_argument (Pair_Term e (use_data_term u)) (address_pair_data (s,d))
+      (generation_predecessor_row_term (Payload_Term s) (Payload_Term d) (site_data_term v a) h)"
+    "environment_value_presents E e" "octets_formed s" "located_at E u d v a"
+    "(151,Pair_Term (generation_source_term e (use_data_term v) (Payload_Term a)) h)
+      \<in>positive_meaning generation_source_system"
+    using holds by (simp only: generation_child_row_equation) blast
+  obtain H where child: "generation_value_presents H h" "generation_at E v a H"
+    using fields(5) by (simp only: generation_core_report_at_source[OF fields(2)]) blast
+  have call: "(44,citation_observation_argument e (use_data_term u) (Payload_Term d) (site_data_term v a))
+      \<in>positive_meaning located_admission_system"
+    using fields(4) by (simp add: located_admission_on_values[OF fields(2)])
+  have coordinates: "octets_formed d" "octets_formed a"
+    using schema_call_formed_target[OF positive_meaning_formed[OF call]] by auto
+  have row: "generation_predecessor_row_presents (s,(d,((v,a),H)))
+      (generation_predecessor_row_term (Payload_Term s) (Payload_Term d) (site_data_term v a) h)"
+    using fields(3) coordinates child(1) by (auto simp: generation_predecessor_row_presents_fields)
+  show "generation_child_row_result t" using fields(1,2,4) row child(2) by blast
+next
+  assume "generation_child_row_result t"
+  then obtain E e u s d v a H row where parts:
+    "t=context_relation_argument (Pair_Term e (use_data_term u)) (address_pair_data (s,d)) row"
+    "environment_value_presents E e" "generation_predecessor_row_presents (s,(d,((v,a),H))) row"
+    "located_at E u d v a" "generation_at E v a H" by blast
+  obtain h where "value": "row=generation_predecessor_row_term (Payload_Term s) (Payload_Term d) (site_data_term v a) h"
+    "octets_formed s" "generation_value_presents H h"
+    using parts(3) by (auto simp: generation_predecessor_row_presents_fields)
+  have report: "(151,Pair_Term (generation_source_term e (use_data_term v) (Payload_Term a)) h)
+      \<in>positive_meaning generation_source_system"
+    using parts(5) by (simp add: generation_core_report_on_values[OF parts(2) "value"(3)])
+  show "(153,t)\<in>positive_meaning generation_source_system"
+    using parts(1,2,4) "value"(1,2) report by (auto simp: generation_child_row_equation)
+qed
+
+corollary generation_child_row_on_values:
+  assumes source: "environment_value_presents E e"
+    and "value": "generation_predecessor_row_presents (s,(d,((v,a),H))) row"
+  shows "(153,context_relation_argument (Pair_Term e (use_data_term u)) (address_pair_data (k,z)) row)
+      \<in>positive_meaning generation_source_system \<longleftrightarrow>
+    k=s \<and> z=d \<and> located_at E u d v a \<and> generation_at E v a H"
+proof -
+  obtain h where fields: "row=generation_predecessor_row_term (Payload_Term s) (Payload_Term d) (site_data_term v a) h"
+    "octets_formed s" "generation_value_presents H h"
+    using "value" by (auto simp: generation_predecessor_row_presents_fields)
+  show ?thesis using fields(2)
+    by (auto simp: generation_child_row_at_source[OF source] fields(1)
+      generation_core_report_on_values[OF source fields(3)])
+qed
+
+lemma generation_child_row_at_fields:
+  assumes source: "environment_value_presents E e" and fields: "generation_fields_at E u r l M p c"
+    and edge: "edge\<in>M" and "value": "generation_predecessor_row_presents row t"
+  shows "(153,context_relation_argument (Pair_Term e (use_data_term u)) (address_pair_data edge) t)
+      \<in>positive_meaning generation_source_system \<longleftrightarrow>
+    row\<in>generation_predecessor_rows E u r \<and> generation_predecessor_socket_row row=edge"
+proof -
+  obtain k z where edge_shape: "edge=(k,z)" by (cases edge)
+  obtain s d v a H where row_shape: "row=(s,(d,((v,a),H)))"
+    by (rule that[of "fst row" "fst (snd row)" "fst (fst (snd (snd row)))"
+      "snd (fst (snd (snd row)))" "snd (snd (snd row))"]) simp
+  have presented: "generation_predecessor_row_presents (s,(d,((v,a),H))) t" using "value" row_shape by simp
+  show ?thesis using edge
+    by (auto simp: edge_shape row_shape generation_child_row_on_values[OF source presented]
+      generation_predecessor_rows_at_source_fields[OF fields])
+qed
+
+lemma generation_predecessor_row_lists:
+  assumes source: "environment_value_presents E e"
+    and fields: "generation_fields_at E u r l (set ms) p c"
+    and rows: "list_all2 generation_predecessor_row_presents Rs qs"
+  shows "(154,context_relation_argument (Pair_Term e (use_data_term u))
+      (data_list_term (map address_pair_data ms)) (data_list_term qs))\<in>positive_meaning generation_source_system
+    \<longleftrightarrow> list_all2 (\<lambda>edge row. row\<in>generation_predecessor_rows E u r \<and>
+      generation_predecessor_socket_row row=edge) ms Rs"
+proof -
+  have first: "list_all2 (\<lambda>edge t. t=address_pair_data edge \<and> edge\<in>set ms) ms (map address_pair_data ms)"
+    by (simp add: list_all2_function_restricted)
+  have ctx_formed: "term_formed (Pair_Term e (use_data_term u))"
+    using environment_value_presents_formed[OF source] by simp
+  show ?thesis by (rule generation_child_rows.readings[OF first rows ctx_formed])
+    (use generation_child_row_at_fields[OF source fields] in blast)
+qed
+
+section \<open>A report enumerates the whole actual predecessor relation\<close>
+
+theorem generation_predecessor_report_on_source:
+  assumes source: "environment_value_presents E e" and native: "generation_at E u r G"
+  shows "(155,Pair_Term (generation_source_term e (use_data_term u) (Payload_Term r)) value)
+      \<in>positive_meaning generation_source_system \<longleftrightarrow>
+    data_collection_presents generation_predecessor_row_presents (generation_predecessor_rows E u r) value"
+proof
+  let ?L="generation_predecessor_rows E u r"
+  assume holds: "(155,Pair_Term (generation_source_term e (use_data_term u) (Payload_Term r)) value)
+      \<in>positive_meaning generation_source_system"
+  obtain a m b q where calls:
+    "(148,generation_fields_argument e (use_data_term u) (Payload_Term r) a m b q)\<in>positive_meaning generation_source_system"
+    "(154,context_relation_argument (Pair_Term e (use_data_term u)) m value)\<in>positive_meaning generation_source_system"
+    using holds by (auto simp: generation_predecessor_report_calls)
+  obtain l ms p c where fields: "m=data_list_term (map address_pair_data ms)" "distinct ms"
+    "generation_fields_at E u r l (set ms) p c"
+    using calls(1) environment_value_presents_unique[OF _ source]
+    by (auto simp: generation_fields_exact dest: injD[OF use_data_term_injective])
+  obtain qs where traversal: "value=data_list_term qs"
+    "list_all2 (\<lambda>x y. (153,context_relation_argument (Pair_Term e (use_data_term u)) x y)
+      \<in>positive_meaning generation_source_system) (map address_pair_data ms) qs"
+    using calls(2) by (auto simp: fields(1) generation_child_rows.exact data_list_term_injective)
+  have recovered: "\<forall>q\<in>set qs. \<exists>row. generation_predecessor_row_presents row q"
+    using list_all2_members[OF traversal(2)] by (auto simp: generation_child_row_exact; blast)
+  obtain Rs where presented: "list_all2 generation_predecessor_row_presents Rs qs"
+    using recovered by (simp only: list_all2_exists_left) blast
+  have linked: "list_all2 (\<lambda>edge row. row\<in>?L \<and> generation_predecessor_socket_row row=edge) ms Rs"
+    using calls(2) by (simp only: fields(1) traversal(1) generation_predecessor_row_lists[OF source fields(3) presented])
+  have bounded: "set Rs\<subseteq>?L" using list_all2_members[OF linked] by blast
+  have mapped: "map generation_predecessor_socket_row Rs=ms"
+  proof (rule nth_equalityI)
+    show "length (map generation_predecessor_socket_row Rs)=length ms"
+      using list_all2_lengthD[OF linked] by simp
+  next
+    fix i assume index: "i<length (map generation_predecessor_socket_row Rs)"
+    show "map generation_predecessor_socket_row Rs!i=ms!i"
+      using linked index by (auto simp: list_all2_conv_all_nth)
+  qed
+  have mapped_distinct: "distinct (map generation_predecessor_socket_row Rs)"
+    using fields(2) by (simp only: mapped)
+  have separate: "distinct Rs" using mapped_distinct by (simp only: distinct_map; blast)
+  have projection: "bij_betw generation_predecessor_socket_row ?L (set ms)"
+    by (rule generation_predecessor_rows_projection[OF native fields(3)])
+  have complete: "set Rs=?L"
+  proof
+    show "set Rs\<subseteq>?L" by (rule bounded)
+    show "?L\<subseteq>set Rs"
+    proof
+      fix row assume member: "row\<in>?L"
+      have edge: "generation_predecessor_socket_row row\<in>set ms"
+        using projection member by (auto simp: bij_betw_def)
+      obtain other where other: "other\<in>set Rs" "generation_predecessor_socket_row other=generation_predecessor_socket_row row"
+        using edge mapped by auto
+      have inside: "other\<in>?L" using bounded other(1) by blast
+      have injective: "inj_on generation_predecessor_socket_row ?L" using projection by (simp add: bij_betw_def)
+      have same: "other=row" by (rule inj_onD[OF injective other(2) inside member])
+      show "row\<in>set Rs" using other(1) same by simp
+    qed
+  qed
+  show "data_collection_presents generation_predecessor_row_presents ?L value"
+    using separate complete presented traversal(1) by (auto simp: data_collection_presents_def)
+next
+  let ?L="generation_predecessor_rows E u r"
+  assume presented: "data_collection_presents generation_predecessor_row_presents ?L value"
+  obtain Rs qs where rows: "distinct Rs" "set Rs=?L" "list_all2 generation_predecessor_row_presents Rs qs"
+    "value=data_list_term qs" using presented by (auto simp: data_collection_presents_def)
+  obtain l M p c where fields: "generation_fields_at E u r l M p c"
+    using native by (cases rule: generation_at.cases) blast
+  have projection: "bij_betw generation_predecessor_socket_row ?L M"
+    by (rule generation_predecessor_rows_projection[OF native fields])
+  let ?ms="map generation_predecessor_socket_row Rs"
+  have keys: "distinct ?ms" and domain: "set ?ms=M"
+    using rows(1,2) projection by (auto simp: distinct_map bij_betw_def)
+  have fields': "generation_fields_at E u r l (set ?ms) p c" using fields domain by simp
+  have linked: "list_all2 (\<lambda>edge row. row\<in>?L \<and> generation_predecessor_socket_row row=edge) ?ms Rs"
+    using rows(2) by (simp add: list_all2_map1 list_all2_same)
+  have traversal: "(154,context_relation_argument (Pair_Term e (use_data_term u))
+      (data_list_term (map address_pair_data ?ms)) value)\<in>positive_meaning generation_source_system"
+    using linked by (simp only: rows(4) generation_predecessor_row_lists[OF source fields' rows(3)])
+  obtain a b q where "values": "target_value_presents l a" "target_value_presents p b" "target_value_presents c q"
+    using generation_fields_formed[OF fields] target_value_presents_total by blast
+  have fields_admitted: "(148,generation_fields_argument e (use_data_term u) (Payload_Term r) a
+      (data_list_term (map address_pair_data ?ms)) b q)\<in>positive_meaning generation_source_system"
+    using keys fields' by (simp only: generation_fields_on_rows[OF source "values"]; blast)
+  have source_admitted: "(152,generation_source_term e (use_data_term u) (Payload_Term r))
+      \<in>positive_meaning generation_source_system"
+    using native by (auto simp: generation_source_at_source[OF source])
+  show "(155,Pair_Term (generation_source_term e (use_data_term u) (Payload_Term r)) value)
+      \<in>positive_meaning generation_source_system"
+    using source_admitted fields_admitted traversal by (auto simp: generation_predecessor_report_calls)
+qed
+
+theorem generation_predecessor_report_exact:
+  "(155,t)\<in>positive_meaning generation_source_system \<longleftrightarrow>
+    (\<exists>z. generation_predecessor_report_presents z t)"
+proof
+  assume holds: "(155,t)\<in>positive_meaning generation_source_system"
+  obtain source "value" where shape: "t=Pair_Term source value"
+    and admitted: "(152,source)\<in>positive_meaning generation_source_system"
+    using holds by (auto simp: generation_predecessor_report_calls)
+  obtain E u r G where reading: "generation_source_presents ((E,(u,r)),G) source"
+    using admitted by (auto simp: generation_source_exact)
+  have native: "generation_at E u r G" using reading by (simp add: generation_source_presents_def)
+  obtain e where input: "source=generation_source_term e (use_data_term u) (Payload_Term r)"
+    "environment_value_presents E e"
+    using reading by (auto simp: generation_source_presents_def source_root_presents_fields)
+  have rows: "data_collection_presents generation_predecessor_row_presents (generation_predecessor_rows E u r) value"
+    using holds by (simp only: shape input(1) generation_predecessor_report_on_source[OF input(2) native])
+  show "\<exists>z. generation_predecessor_report_presents z t"
+    by (rule exI[of _ "(((E,(u,r)),G),generation_predecessor_rows E u r)"])
+      (use reading rows shape in \<open>auto simp: generation_predecessor_report_presents_def factor_pair_presents_def\<close>)
+next
+  assume "\<exists>z. generation_predecessor_report_presents z t"
+  then obtain E u r G source "value" where fields: "t=Pair_Term source value"
+    "generation_source_presents ((E,(u,r)),G) source"
+    "data_collection_presents generation_predecessor_row_presents (generation_predecessor_rows E u r) value"
+    by (auto simp: generation_predecessor_report_presents_def factor_pair_presents_def)
+  have native: "generation_at E u r G" using fields(2) by (simp add: generation_source_presents_def)
+  obtain e where input: "source=generation_source_term e (use_data_term u) (Payload_Term r)"
+    "environment_value_presents E e"
+    using fields(2) by (auto simp: generation_source_presents_def source_root_presents_fields)
+  show "(155,t)\<in>positive_meaning generation_source_system"
+    using fields(3) by (simp only: fields(1) input(1) generation_predecessor_report_on_source[OF input(2) native])
+qed
+
+text \<open>
+  The whole parent is admitted before its predecessor report. Its complete
+  socket graph is in bijection with the actual predecessor rows. A report
+  can enumerate those rows in any order; projecting that enumeration gives
+  an admitted complete socket enumeration in the same order.
+
+  The two traversal contracts retain every corresponding row and its actual
+  source context. Exact child cores do not replace cited destinations. Empty
+  reports still admit the parent and its empty predecessor family. Missing,
+  repeated, and unrelated rows cannot satisfy the complete report class.
+\<close>
+
+end
